grammatik/Grammatik.lean
@@ -127,3 +127,5 @@ import Grammatik.KostenG
 import Grammatik.KostenGZeuge
 import Grammatik.AuditFinal
 import Grammatik.Parser.Lexer
+import Grammatik.Parser.Ausdruck
+import Grammatik.Parser.AusdruckProben
